More progress on the SHA block_data_order proof

sha/sha_lemmas.v
@@ -1407,3 +1407,156 @@ clear - H2; revert contents H2; induction (Z.to_nat i); intros; destruct content
 simpl in *; try omega; auto.
 apply IHn. omega.
 Qed.
+
+Definition f_upto {t} (f: Z -> reptype t) (bound: Z) (i: Z) : reptype t :=
+ if zlt i bound then f i else default_val t.
+
+Lemma array_at_f_upto_lo:
+  forall t sh contents lo hi, 
+  array_at t sh (f_upto contents lo) lo hi = array_at_ t sh lo hi.
+Proof.
+intros; apply array_at_ext; intros.
+unfold f_upto; if_tac; auto. omega.
+Qed.
+
+Lemma and_mone':
+ forall x, Int.and x (Int.repr (-1)) = x.
+Proof.
+apply Int.and_mone.
+Qed.
+
+Lemma Sigma_1_eq: forall f_,
+  Sigma_1 f_ =
+            (Int.xor
+              (Int.xor
+                 (Int.or (Int.shl f_ (Int.repr 26))
+                    (Int.shru (Int.and f_ (Int.repr (-1)))
+                       (Int.sub (Int.repr 32) (Int.repr 26))))
+                 (Int.or (Int.shl f_ (Int.repr 21))
+                    (Int.shru (Int.and f_ (Int.repr (-1)))
+                       (Int.sub (Int.repr 32) (Int.repr 21)))))
+              (Int.or (Int.shl f_ (Int.repr 7))
+                 (Int.shru (Int.and f_ (Int.repr (-1)))
+                    (Int.sub (Int.repr 32) (Int.repr 7))))).
+Proof.
+intros.
+unfold Sigma_1, Sh.
+repeat rewrite and_mone'.
+repeat rewrite <- Int.or_ror by reflexivity.
+change (Int.sub (Int.repr 32) (Int.repr 26)) with (Int.repr 6).
+change (Int.sub (Int.repr 32) (Int.repr 21)) with (Int.repr 11).
+change (Int.sub (Int.repr 32) (Int.repr 7)) with (Int.repr 25).
+reflexivity.
+Qed.
+
+Lemma  Sigma_0_eq: forall b_,
+   Sigma_0 b_ = 
+      (Int.xor
+        (Int.xor
+           (Int.or (Int.shl b_ (Int.repr 30))
+              (Int.shru (Int.and b_ (Int.repr (-1)))
+                 (Int.sub (Int.repr 32) (Int.repr 30))))
+           (Int.or (Int.shl b_ (Int.repr 19))
+              (Int.shru (Int.and b_ (Int.repr (-1)))
+                 (Int.sub (Int.repr 32) (Int.repr 19)))))
+        (Int.or (Int.shl b_ (Int.repr 10))
+           (Int.shru (Int.and b_ (Int.repr (-1)))
+              (Int.sub (Int.repr 32) (Int.repr 10))))).
+Proof.
+intros.
+unfold Sigma_0, Sh.
+repeat rewrite and_mone'.
+repeat rewrite <- Int.or_ror by reflexivity.
+change (Int.sub (Int.repr 32) (Int.repr 19)) with (Int.repr 13).
+change (Int.sub (Int.repr 32) (Int.repr 10)) with (Int.repr 22).
+change (Int.sub (Int.repr 32) (Int.repr 30)) with (Int.repr 2).
+reflexivity.
+Qed.
+
+Lemma Ch_eq: forall f_ g_ h_,
+  Ch f_ g_ h_ =
+        (Int.xor (Int.and f_ g_) (Int.and (Int.not f_) h_)).
+Proof. reflexivity.
+Qed.
+
+Lemma Maj_eq:
+  forall b c d, 
+  Maj b c d =
+  (Int.xor (Int.xor (Int.and b c) (Int.and b d)) (Int.and c d)).
+Proof.
+intros.
+unfold Maj.
+rewrite (Int.xor_commut) at 1.
+rewrite Int.xor_assoc. auto.
+Qed.
+
+Lemma sigma_1_eq:
+ forall s, sigma_1 s = 
+   Int.xor
+     (Int.xor
+        (Int.or (Int.shl s (Int.repr 15))
+           (Int.shru s (Int.sub (Int.repr 32) (Int.repr 15))))
+        (Int.or (Int.shl s (Int.repr 13))
+           (Int.shru s (Int.sub (Int.repr 32) (Int.repr 13)))))
+  (Int.shru s (Int.repr 10)).
+Proof.
+intros.
+unfold sigma_1.
+f_equal. f_equal.
+repeat rewrite <- Int.or_ror by reflexivity.
+unfold Sh. f_equal.
+repeat rewrite <- Int.or_ror by reflexivity.
+unfold Sh. f_equal.
+Qed.
+
+Lemma sigma_0_eq:
+ forall s, sigma_0 s = 
+  Int.xor
+   (Int.xor
+     (Int.or (Int.shl s (Int.repr 25))
+        (Int.shru s (Int.sub (Int.repr 32) (Int.repr 25))))
+     (Int.or (Int.shl s (Int.repr 14))
+        (Int.shru s (Int.sub (Int.repr 32) (Int.repr 14)))))
+   (Int.shru s (Int.repr 3)).
+Proof.
+intros.
+unfold sigma_0.
+f_equal. f_equal.
+repeat rewrite <- Int.or_ror by reflexivity.
+unfold Sh. f_equal.
+repeat rewrite <- Int.or_ror by reflexivity.
+unfold Sh. f_equal.
+Qed.
+
+
+(* MOVE THESE TO FLOYD *)
+
+Lemma assert_LOCAL:
+ forall Q1 Espec Delta P Q R c Post,
+    PROPx P (LOCALx (tc_environ Delta :: Q) (SEPx R)) |-- local Q1 ->
+   @semax Espec Delta (PROPx P (LOCALx (Q1::Q) (SEPx R))) c Post ->
+   @semax Espec Delta (PROPx P (LOCALx Q (SEPx R))) c Post.
+Proof.
+intros.
+eapply semax_pre; try apply H0.
+rewrite <- (insert_local Q1); apply andp_right; auto.
+rewrite <- insert_local; apply andp_left2; auto.
+Qed.
+
+Lemma drop_LOCAL:
+  forall (n: nat) Espec Delta P Q R c Post,
+   @semax Espec Delta (PROPx P (LOCALx (delete_nth n Q) (SEPx R))) c Post ->
+   @semax Espec Delta (PROPx P (LOCALx Q (SEPx R))) c Post.
+Proof.
+intros.
+eapply semax_pre; try apply H.
+rewrite <- insert_local. apply andp_left2.
+apply andp_derives; auto.
+apply andp_derives; auto.
+intro rho; unfold local, lift1; unfold_lift. apply prop_derives; simpl.
+clear.
+revert Q; induction n; destruct Q; simpl; intros; intuition.
+Qed.
+
+
+
