sha/verif_sha_bdo3.v
@@ -5,77 +5,6 @@ Require Import sha.sha_lemmas.
 Require Import sha.spec_sha.
 Local Open Scope logic.
 
-Lemma and_mone':
- forall x, Int.and x (Int.repr (-1)) = x.
-Proof.
-apply Int.and_mone.
-Qed.
-
-Lemma Sigma_1_eq: forall f_,
-  Sigma_1 f_ =
-            (Int.xor
-              (Int.xor
-                 (Int.or (Int.shl f_ (Int.repr 26))
-                    (Int.shru (Int.and f_ (Int.repr (-1)))
-                       (Int.sub (Int.repr 32) (Int.repr 26))))
-                 (Int.or (Int.shl f_ (Int.repr 21))
-                    (Int.shru (Int.and f_ (Int.repr (-1)))
-                       (Int.sub (Int.repr 32) (Int.repr 21)))))
-              (Int.or (Int.shl f_ (Int.repr 7))
-                 (Int.shru (Int.and f_ (Int.repr (-1)))
-                    (Int.sub (Int.repr 32) (Int.repr 7))))).
-Proof.
-intros.
-unfold Sigma_1, Sh.
-repeat rewrite and_mone'.
-repeat rewrite <- Int.or_ror by reflexivity.
-change (Int.sub (Int.repr 32) (Int.repr 26)) with (Int.repr 6).
-change (Int.sub (Int.repr 32) (Int.repr 21)) with (Int.repr 11).
-change (Int.sub (Int.repr 32) (Int.repr 7)) with (Int.repr 25).
-reflexivity.
-Qed.
-
-Lemma  Sigma_0_eq: forall b_,
-   Sigma_0 b_ = 
-      (Int.xor
-        (Int.xor
-           (Int.or (Int.shl b_ (Int.repr 30))
-              (Int.shru (Int.and b_ (Int.repr (-1)))
-                 (Int.sub (Int.repr 32) (Int.repr 30))))
-           (Int.or (Int.shl b_ (Int.repr 19))
-              (Int.shru (Int.and b_ (Int.repr (-1)))
-                 (Int.sub (Int.repr 32) (Int.repr 19)))))
-        (Int.or (Int.shl b_ (Int.repr 10))
-           (Int.shru (Int.and b_ (Int.repr (-1)))
-              (Int.sub (Int.repr 32) (Int.repr 10))))).
-Proof.
-intros.
-unfold Sigma_0, Sh.
-repeat rewrite and_mone'.
-repeat rewrite <- Int.or_ror by reflexivity.
-change (Int.sub (Int.repr 32) (Int.repr 19)) with (Int.repr 13).
-change (Int.sub (Int.repr 32) (Int.repr 10)) with (Int.repr 22).
-change (Int.sub (Int.repr 32) (Int.repr 30)) with (Int.repr 2).
-reflexivity.
-Qed.
-
-Lemma Ch_eq: forall f_ g_ h_,
-  Ch f_ g_ h_ =
-        (Int.xor (Int.and f_ g_) (Int.and (Int.not f_) h_)).
-Proof. reflexivity.
-Qed.
-
-Lemma Maj_eq:
-  forall b c d, 
-  Maj b c d =
-  (Int.xor (Int.xor (Int.and b c) (Int.and b d)) (Int.and c d)).
-Proof.
-intros.
-unfold Maj.
-rewrite (Int.xor_commut) at 1.
-rewrite Int.xor_assoc. auto.
-Qed.
-
 Lemma rearrange_aux:
  forall h f c k l,
  Int.add (Int.add (Int.add (Int.add h f) c) k) l =
@@ -298,18 +227,6 @@ rewrite <- HDelta''; unfold Delta'.
 clear HDelta' Delta' HDelta'' Delta.
 subst regs'.
 simple apply rearrange_aux2; assumption. 
-Qed.
-
-
-Definition f_upto {t} (f: Z -> reptype t) (bound: Z) (i: Z) : reptype t :=
- if zlt i bound then f i else default_val t.
-
-Lemma array_at_f_upto_lo:
-  forall t sh contents lo hi, 
-  array_at t sh (f_upto contents lo) lo hi = array_at_ t sh lo hi.
-Proof.
-intros; apply array_at_ext; intros.
-unfold f_upto; if_tac; auto. omega.
 Qed.
 
 Lemma loop1_aux_lemma1:
