sha/bdo_lemmas.v
@@ -1,0 +1,288 @@
+Require Import proofauto.
+Require Import sha.SHA256.
+Require Import sha.spec_sha.
+Require Import sha.sha_lemmas.
+
+Lemma generate_word_lemma1:
+  forall b n, length b = LBLOCK ->
+   firstn LBLOCK (rev (generate_word (rev b) n)) = b.
+Proof.
+intros.
+change (rev b) with (nil ++ rev b).
+forget (@nil int) as a.
+Transparent generate_word.
+revert a; induction n; intro.
+unfold generate_word.
+rewrite rev_app_distr.
+rewrite rev_involutive.
+rewrite firstn_app1 by omega.
+rewrite firstn_same; auto; omega.
+unfold generate_word; fold generate_word.
+change (W (a ++ rev b) :: a ++ rev b) with 
+      ((W (a ++ rev b) ::a) ++ rev b).
+apply IHn.
+Opaque generate_word.
+Qed.
+
+Lemma length_generate_word: forall b n,
+  length (generate_word b n) = (length b + n)%nat.
+Proof.
+Transparent generate_word.
+intros.
+revert b; induction n; intros; simpl.
+unfold generate_word; fold generate_word.
+omega.
+unfold generate_word; fold generate_word.
+rewrite IHn.
+simpl. omega.
+Opaque generate_word.
+Qed.
+
+Lemma and_mod_15_lem:
+ forall (n: Z), 0 <= Int.signed (Int.and (Int.repr n) (Int.repr 15)) < 16.
+Proof.
+intro n.
+unfold Int.and.
+rewrite (Int.unsigned_repr 15) by repable_signed.
+change 15 with (Z.ones 4).
+assert (0 <= Z.land (Int.unsigned (Int.repr n)) (Z.ones 4) < 16).
+rewrite Z.land_ones.
+apply Z.mod_bound_pos. 
+apply Int.unsigned_range. clear; omega. clear; omega.
+rewrite Int.signed_repr; auto.
+repable_signed.
+Qed.
+
+Transparent generate_word.
+
+Lemma nth_generate_word_S:
+  forall k i n b', 
+   nth (i+k) (generate_word b' (n+k)) = nth i (generate_word b' n).
+Proof.
+induction k; intros.
+repeat rewrite plus_0_r. auto.
+replace (n + S k)%nat with (S (n + k))%nat by omega.
+unfold generate_word; fold generate_word.
+replace (i + S k)%nat with (S i + k)%nat by omega.
+rewrite IHk by (simpl; omega).
+clear IHk.
+revert i b' ; induction n; intros.
+unfold generate_word; fold generate_word.
+extensionality d; reflexivity.
+unfold generate_word; fold generate_word.
+apply IHn.
+Qed.
+
+Lemma generate_word_small:
+  forall i b n,
+           length b = 16%nat ->
+           (i < length b)%nat -> 
+           nth i (rev (generate_word (rev b) n)) = nth i b.
+Proof.
+intros.
+extensionality d.
+rewrite <- (nth_firstn_low _ _ LBLOCK).
+rewrite (generate_word_lemma1 b n H).
+auto.
+rewrite rev_length, length_generate_word, rev_length, H.
+change LBLOCK with 16%nat. omega.
+Qed.
+Opaque generate_word.
+
+Definition Xarray (b: list int) (i j: Z) :=
+   tuints (rev (generate_word (rev b) 48)) (i-16+(j-i) mod 16).
+
+Lemma array_at_Xarray:
+ forall b, 
+    length b = 16%nat ->
+    array_at tuint Tsh (Xarray b 16) 0 16 = array_at tuint Tsh (tuints b) 0 16.
+Proof.
+intros.
+apply array_at_ext; intros j ?.
+unfold Xarray, tuints, ZnthV.
+change (16-16)%Z with 0%Z.
+rewrite Z.add_0_l.
+assert (0 <= (j-16)mod 16 < 16)%Z by (apply Z.mod_pos_bound; omega).
+rewrite if_false by omega.
+rewrite if_false by omega.
+rewrite Zminus_mod. rewrite Z.mod_same by omega.
+rewrite Z.sub_0_r. rewrite Z.mod_mod by omega.
+rewrite Z.mod_small by auto.
+assert (Z.to_nat j < length b)%nat 
+ by (apply Nat2Z.inj_lt; rewrite Z2Nat.id by omega; rewrite H; apply H0).
+rewrite (@nth_map' int val _ _ Int.zero).
+rewrite (@nth_map' int val _ _ Int.zero) by auto.
+f_equal.
+rewrite (generate_word_small (Z.to_nat j)); auto.
+rewrite rev_length, length_generate_word, rev_length; omega.
+Qed.
+
+Lemma X_subscript_aux:
+  forall n (b: list int) (i: nat), 
+  (16 <= Z.of_nat i < 64)%Z ->
+  length b = LBLOCK ->
+  is_int
+  (Xarray b (Z.of_nat i)
+    (Int.signed (Int.and (Int.repr (Z.of_nat i + n)) (Int.repr 15)))).
+Proof.
+intros.
+unfold Xarray, tuints,ZnthV.
+ pose proof  (and_mod_15_lem (Z.of_nat i + n)).
+ forget (Int.signed (Int.and (Int.repr (Z.of_nat i + n)) (Int.repr 15))) as k.
+ assert (0 <= (k - Z.of_nat i) mod 16 < 16)%Z
+  by ( apply  Z.mod_pos_bound; omega).
+ rewrite if_false by omega.
+ rewrite (@nth_map' int val _ _ Int.zero). apply I.
+ rewrite rev_length, length_generate_word, rev_length, H0.
+ change (LBLOCK+48)%nat with 64%nat.
+ change 64%nat with (Z.to_nat 64).
+ apply Z2Nat.inj_lt; omega.
+Qed.
+
+Definition nthB (b: list int) (i: nat) (n: Z) :=
+  nth (Z.to_nat (Z.of_nat i - 16 + n)) (rev (generate_word (rev b) 48)) Int.zero.
+
+
+Lemma extract_from_b:
+  forall b i n,
+    length b = 16%nat ->
+    (16 <= i < 64)%nat ->
+    (0 <= n < 16)%Z ->
+    (Xarray b (Z.of_nat i) ((Z.of_nat i + n) mod 16) = Vint (nthB b i n))%Z.
+Proof.
+intros.
+assert (0 <= (Z.of_nat i + n) mod 16 < 16)%Z by (apply Z_mod_lt; clear; omega).
+unfold Xarray, tuints, ZnthV.
+replace (((Z.of_nat i + n) mod 16 - Z.of_nat i) mod 16)%Z 
+  with (n mod 16)%Z
+ by (rewrite Zminus_mod, Zmod_mod, <- Zminus_mod; f_equal; omega).
+ rewrite Z.mod_small by omega.
+rewrite if_false by omega.
+rewrite (@nth_map' int val _ _ Int.zero)
+ by (rewrite rev_length, length_generate_word, rev_length, H;
+      change (16+48)%nat with (Z.to_nat 64);
+      apply Z2Nat.inj_lt; omega).
+unfold nthB.
+reflexivity.
+Qed.
+
+Lemma X_subscript_aux2:
+  forall n, 0 <= n < Int.max_unsigned -> 
+        Int.signed (Int.and (Int.repr n) (Int.repr 15)) = n mod 16.
+Proof.
+intros. unfold Int.and. rewrite (Int.unsigned_repr 15) by repable_signed.
+ change 15 with (Z.ones 4). rewrite Z.land_ones by repable_signed.
+ rewrite Int.unsigned_repr by repable_signed.
+ rewrite Int.signed_repr. f_equal.
+ destruct H.
+ pose proof (Z.mod_bound_pos n 16 H).
+ change (2^4) with 16. repable_signed. 
+Qed.
+
+
+Definition c64 := 64%nat.  Global Opaque c64.
+Definition c48 := 48%nat.  Global Opaque c48.
+
+
+Transparent generate_word.
+Lemma generate_word_plus:
+  forall msg a b, (16 <= length msg)%nat ->
+         generate_word msg (a+b) = generate_word (generate_word msg a) b.
+Proof.
+intros msg a b.
+revert msg b; induction a; simpl; intros.
+unfold generate_word; fold generate_word.
+auto.
+unfold generate_word; fold generate_word.
+rewrite IHa by (simpl; omega).
+auto.
+Qed.
+
+Lemma nth_rev_generate_word:
+ forall i b,
+   length b = LBLOCK -> 
+   (LBLOCK <= i < 64)%nat ->
+    nth i (rev (generate_word (rev b) 48)) Int.zero =
+  Int.add (nthB b i 0)
+    (Int.add (Int.add (sigma_0 (nthB b i 1)) (sigma_1 (nthB b i 14)))
+       (nthB b i 9)).
+Proof.
+intros.
+unfold nthB.
+rewrite <- rev_length in H.
+forget (rev b) as b'.
+clear b.
+change LBLOCK with 16%nat in *.
+assert (length (generate_word b' 48) = 64)%nat 
+ by (rewrite length_generate_word, H; reflexivity).
+rewrite rev_nth by omega.
+repeat rewrite rev_nth
+ by (rewrite H1; change 64%nat with (Z.to_nat 64); apply Z2Nat.inj_lt; omega).
+rewrite H1.
+rewrite <- (plus_0_l (64 - S i)).
+assert (48 = (i - 16) + 1 + (64 - S i))%nat by (clear - H0; omega).
+rewrite H2 at 2.
+rewrite nth_generate_word_S.
+rewrite generate_word_plus by omega.
+unfold generate_word at 1. 
+unfold nth at 1.
+assert (forall n:nat, (n < 16) ->
+    ((64 - S (Z.to_nat (Z.of_nat i - 16 + Z.of_nat n))) =
+      (16-n) + (48 - S (Z.to_nat (Z.of_nat i - 16)))))%nat.
+clear - H0.
+intros.
+rewrite Z2Nat.inj_add by omega.
+rewrite Nat2Z.id.
+rewrite Z2Nat.inj_sub by omega.
+rewrite Nat2Z.id.
+change (Z.to_nat 16) with 16%nat.
+omega.
+change 0%Z with (Z.of_nat 0); rewrite H3 by (clear; omega).
+change 1%Z with (Z.of_nat 1); rewrite H3 by (clear; omega).
+change 14%Z with (Z.of_nat 14); rewrite H3 by (clear; omega).
+change 9%Z with (Z.of_nat 9); rewrite H3 by (clear; omega).
+clear H3.
+assert (48 = S (Z.to_nat (Z.of_nat i - 16)) + (48 - S (Z.to_nat (Z.of_nat i - 16))))%nat.
+clear - H0.
+rewrite Z2Nat.inj_sub by omega.
+rewrite Nat2Z.id.
+change (Z.to_nat 16) with 16%nat.
+omega.
+pattern (generate_word b' 48).
+rewrite H3 at 1.
+repeat rewrite nth_generate_word_S.
+rewrite Z2Nat.inj_sub by omega.
+rewrite Nat2Z.id.
+change (Z.to_nat 16) with 16%nat.
+simpl.
+change (nth 16) with (@nth int (15+1)).
+change (nth 15) with (@nth int (14+1)).
+change (nth 2) with (@nth int (1+1)).
+change (nth 7) with (@nth int (6+1)).
+replace (S (i-16)) with ((i-16)+1)%nat by omega.
+repeat rewrite nth_generate_word_S.
+assert (length (generate_word b' (i-16)) >= 16)%nat.
+rewrite length_generate_word, H; omega.
+clear - H4.
+forget (generate_word b' (i-16)) as s.
+rename H4 into H.
+do 16 (destruct s; [simpl in H; omega | ]).
+simpl.
+rewrite <- Int.add_assoc.
+rewrite Int.add_commut.
+f_equal.
+rewrite Int.add_commut.
+rewrite <- Int.add_assoc.
+auto.
+Qed.
+Opaque generate_word.
+
+Lemma nth_error_nth:
+  forall A (d: A) i al, (i < length al)%nat -> nth_error al i = Some (nth i al d).
+Proof.
+induction i; destruct al; simpl; intros; auto.
+inv H.
+inv H.
+apply IHi; omega.
+Qed.
+
