sha/verif_sha_bdo5.v
@@ -1,0 +1,363 @@
+Require Import floyd.proofauto.
+Require Import sha.sha.
+Require Import sha.SHA256.
+Require Import sha.spec_sha.
+Require Import sha.sha_lemmas.
+Require Import sha.bdo_lemmas.
+Local Open Scope logic.
+
+Definition rearrange_regs2c := 
+     Ssequence (Sset _h (Etempvar _g tuint))
+        (Ssequence (Sset _g (Etempvar _f tuint))
+           (Ssequence (Sset _f (Etempvar _e tuint))
+              (Ssequence
+                 (Sset _e
+                    (Ebinop Oadd (Etempvar _d tuint) (Etempvar _T1 tuint)
+                       tuint))
+                 (Ssequence (Sset _d (Etempvar _c tuint))
+                    (Ssequence (Sset _c (Etempvar _b tuint))
+                       (Ssequence (Sset _b (Etempvar _a tuint))
+                          (Sset _a
+                             (Ebinop Oadd (Etempvar _T1 tuint)
+                                (Etempvar _T2 tuint) tuint)))))))).
+
+Definition rearrange_regs2b :=
+Ssequence
+  (Sset _T1
+     (Ebinop Oadd (Etempvar _T1 tuint)
+        (Ebinop Oadd
+           (Ebinop Oadd
+              (Ebinop Oadd (Etempvar _h tuint)
+                 (Ebinop Oxor
+                    (Ebinop Oxor
+                       (Ebinop Oor
+                          (Ebinop Oshl (Etempvar _e tuint)
+                             (Econst_int (Int.repr 26) tint) tuint)
+                          (Ebinop Oshr
+                             (Ebinop Oand (Etempvar _e tuint)
+                                (Econst_int (Int.repr (-1)) tuint) tuint)
+                             (Ebinop Osub (Econst_int (Int.repr 32) tint)
+                                (Econst_int (Int.repr 26) tint) tint) tuint)
+                          tuint)
+                       (Ebinop Oor
+                          (Ebinop Oshl (Etempvar _e tuint)
+                             (Econst_int (Int.repr 21) tint) tuint)
+                          (Ebinop Oshr
+                             (Ebinop Oand (Etempvar _e tuint)
+                                (Econst_int (Int.repr (-1)) tuint) tuint)
+                             (Ebinop Osub (Econst_int (Int.repr 32) tint)
+                                (Econst_int (Int.repr 21) tint) tint) tuint)
+                          tuint) tuint)
+                    (Ebinop Oor
+                       (Ebinop Oshl (Etempvar _e tuint)
+                          (Econst_int (Int.repr 7) tint) tuint)
+                       (Ebinop Oshr
+                          (Ebinop Oand (Etempvar _e tuint)
+                             (Econst_int (Int.repr (-1)) tuint) tuint)
+                          (Ebinop Osub (Econst_int (Int.repr 32) tint)
+                             (Econst_int (Int.repr 7) tint) tint) tuint)
+                       tuint) tuint) tuint)
+              (Ebinop Oxor
+                 (Ebinop Oand (Etempvar _e tuint) (Etempvar _f tuint) tuint)
+                 (Ebinop Oand (Eunop Onotint (Etempvar _e tuint) tuint)
+                    (Etempvar _g tuint) tuint) tuint) tuint)
+           (Etempvar _Ki tuint) tuint) tuint))
+  (Ssequence
+     (Sset _T2
+        (Ebinop Oadd
+           (Ebinop Oxor
+              (Ebinop Oxor
+                 (Ebinop Oor
+                    (Ebinop Oshl (Etempvar _a tuint)
+                       (Econst_int (Int.repr 30) tint) tuint)
+                    (Ebinop Oshr
+                       (Ebinop Oand (Etempvar _a tuint)
+                          (Econst_int (Int.repr (-1)) tuint) tuint)
+                       (Ebinop Osub (Econst_int (Int.repr 32) tint)
+                          (Econst_int (Int.repr 30) tint) tint) tuint) tuint)
+                 (Ebinop Oor
+                    (Ebinop Oshl (Etempvar _a tuint)
+                       (Econst_int (Int.repr 19) tint) tuint)
+                    (Ebinop Oshr
+                       (Ebinop Oand (Etempvar _a tuint)
+                          (Econst_int (Int.repr (-1)) tuint) tuint)
+                       (Ebinop Osub (Econst_int (Int.repr 32) tint)
+                          (Econst_int (Int.repr 19) tint) tint) tuint) tuint)
+                 tuint)
+              (Ebinop Oor
+                 (Ebinop Oshl (Etempvar _a tuint)
+                    (Econst_int (Int.repr 10) tint) tuint)
+                 (Ebinop Oshr
+                    (Ebinop Oand (Etempvar _a tuint)
+                       (Econst_int (Int.repr (-1)) tuint) tuint)
+                    (Ebinop Osub (Econst_int (Int.repr 32) tint)
+                       (Econst_int (Int.repr 10) tint) tint) tuint) tuint)
+              tuint)
+           (Ebinop Oxor
+              (Ebinop Oxor
+                 (Ebinop Oand (Etempvar _a tuint) (Etempvar _b tuint) tuint)
+                 (Ebinop Oand (Etempvar _a tuint) (Etempvar _c tuint) tuint)
+                 tuint)
+              (Ebinop Oand (Etempvar _b tuint) (Etempvar _c tuint) tuint)
+              tuint) tuint))
+       rearrange_regs2c).
+
+Definition bdo_loop2_body :=
+  (Ssequence
+     (Sset _s0
+        (Ederef
+           (Ebinop Oadd (Evar _X (tarray tuint 16))
+              (Ebinop Oand
+                 (Ebinop Oadd (Etempvar _i tint)
+                    (Econst_int (Int.repr 1) tint) tint)
+                 (Econst_int (Int.repr 15) tint) tint) (tptr tuint)) tuint))
+     (Ssequence
+        (Sset _s0
+           (Ebinop Oxor
+              (Ebinop Oxor
+                 (Ebinop Oor
+                    (Ebinop Oshl (Etempvar _s0 tuint)
+                       (Econst_int (Int.repr 25) tint) tuint)
+                    (Ebinop Oshr
+                       (Ebinop Oand (Etempvar _s0 tuint)
+                          (Econst_int (Int.repr (-1)) tuint) tuint)
+                       (Ebinop Osub (Econst_int (Int.repr 32) tint)
+                          (Econst_int (Int.repr 25) tint) tint) tuint) tuint)
+                 (Ebinop Oor
+                    (Ebinop Oshl (Etempvar _s0 tuint)
+                       (Econst_int (Int.repr 14) tint) tuint)
+                    (Ebinop Oshr
+                       (Ebinop Oand (Etempvar _s0 tuint)
+                          (Econst_int (Int.repr (-1)) tuint) tuint)
+                       (Ebinop Osub (Econst_int (Int.repr 32) tint)
+                          (Econst_int (Int.repr 14) tint) tint) tuint) tuint)
+                 tuint)
+              (Ebinop Oshr (Etempvar _s0 tuint)
+                 (Econst_int (Int.repr 3) tint) tuint) tuint))
+        (Ssequence
+           (Sset _s1
+              (Ederef
+                 (Ebinop Oadd (Evar _X (tarray tuint 16))
+                    (Ebinop Oand
+                       (Ebinop Oadd (Etempvar _i tint)
+                          (Econst_int (Int.repr 14) tint) tint)
+                       (Econst_int (Int.repr 15) tint) tint) (tptr tuint))
+                 tuint))
+           (Ssequence
+              (Sset _s1
+                 (Ebinop Oxor
+                    (Ebinop Oxor
+                       (Ebinop Oor
+                          (Ebinop Oshl (Etempvar _s1 tuint)
+                             (Econst_int (Int.repr 15) tint) tuint)
+                          (Ebinop Oshr
+                             (Ebinop Oand (Etempvar _s1 tuint)
+                                (Econst_int (Int.repr (-1)) tuint) tuint)
+                             (Ebinop Osub (Econst_int (Int.repr 32) tint)
+                                (Econst_int (Int.repr 15) tint) tint) tuint)
+                          tuint)
+                       (Ebinop Oor
+                          (Ebinop Oshl (Etempvar _s1 tuint)
+                             (Econst_int (Int.repr 13) tint) tuint)
+                          (Ebinop Oshr
+                             (Ebinop Oand (Etempvar _s1 tuint)
+                                (Econst_int (Int.repr (-1)) tuint) tuint)
+                             (Ebinop Osub (Econst_int (Int.repr 32) tint)
+                                (Econst_int (Int.repr 13) tint) tint) tuint)
+                          tuint) tuint)
+                    (Ebinop Oshr (Etempvar _s1 tuint)
+                       (Econst_int (Int.repr 10) tint) tuint) tuint))
+              (Ssequence
+                 (Sset _T1
+                    (Ederef
+                       (Ebinop Oadd (Evar _X (tarray tuint 16))
+                          (Ebinop Oand (Etempvar _i tint)
+                             (Econst_int (Int.repr 15) tint) tint)
+                          (tptr tuint)) tuint))
+                 (Ssequence
+                    (Sset _t
+                       (Ederef
+                          (Ebinop Oadd (Evar _X (tarray tuint 16))
+                             (Ebinop Oand
+                                (Ebinop Oadd (Etempvar _i tint)
+                                   (Econst_int (Int.repr 9) tint) tint)
+                                (Econst_int (Int.repr 15) tint) tint)
+                             (tptr tuint)) tuint))
+                    (Ssequence
+                       (Sset _T1
+                          (Ebinop Oadd (Etempvar _T1 tuint)
+                             (Ebinop Oadd
+                                (Ebinop Oadd (Etempvar _s0 tuint)
+                                   (Etempvar _s1 tuint) tuint)
+                                (Etempvar _t tuint) tuint) tuint))
+                       (Ssequence
+                          (Sassign
+                             (Ederef
+                                (Ebinop Oadd (Evar _X (tarray tuint 16))
+                                   (Ebinop Oand (Etempvar _i tint)
+                                      (Econst_int (Int.repr 15) tint) tint)
+                                   (tptr tuint)) tuint) (Etempvar _T1 tuint))
+                          (Ssequence
+                             (Sset _Ki
+                                (Ederef
+                                   (Ebinop Oadd
+                                      (Evar _K256 (tarray tuint 64))
+                                      (Etempvar _i tint) (tptr tuint)) tuint))
+                             rearrange_regs2b))))))))).
+
+Definition block_data_order_loop2 := 
+   nth 1 (loops (fn_body f_sha256_block_data_order)) Sskip.
+
+Opaque K.
+
+Lemma rearrange_regs2c_proof:
+ forall (Espec : OracleKind)
+   (bb : list int) (ctx : val) ( regs : list int) (i : nat)
+   (regs': registers) (a b c d e f g h: int),
+  length bb = LBLOCK ->
+  (LBLOCK <= i < c64)%nat ->
+  16 <= Z.of_nat i < 64 ->
+  rnd_64 regs K (firstn i (rev (generate_word (rev bb) c48))) =
+  [a, b, c, d, e, f, g, h] ->
+semax
+  (initialized _T2
+     (initialized _Ki
+        (initialized _T1
+           (initialized _t (initialized _s1 (initialized _s0 Delta_loop1))))))
+  (PROP  ()
+   LOCAL  (`(eq (Vint (Int.add (Sigma_0 a) (Maj a b c)))) (eval_id _T2);
+   `(eq
+       (Vint
+          (Int.add
+             (Int.add (nthB bb i 0)
+                (Int.add
+                   (Int.add (sigma_0 (nthB bb i 1)) (sigma_1 (nthB bb i 14)))
+                   (nthB bb i 9)))
+             (Int.add (Int.add (Int.add h (Sigma_1 e)) (Ch e f g))
+                (nth i K Int.zero))))) (eval_id _T1);
+   `(eq (Vint (nth i K Int.zero))) (eval_id _Ki); `(eq ctx) (eval_id _ctx);
+   `(eq (Vint (Int.repr (Z.of_nat i)))) (eval_id _i);
+   `(eq [Vint a, Vint b, Vint c, Vint d, Vint e, Vint f, Vint g, Vint h])
+     (`cons (eval_id _a)
+        (`cons (eval_id _b)
+           (`cons (eval_id _c)
+              (`cons (eval_id _d)
+                 (`cons (eval_id _e)
+                    (`cons (eval_id _f)
+                       (`cons (eval_id _g) (`cons (eval_id _h) `[])))))))))
+   SEP 
+   (`(array_at tuint Tsh (tuints K) 0 (Zlength K))
+      (eval_var _K256 (tarray tuint 64));
+   `(array_at tuint Tsh
+       (upd (Xarray bb (Z.of_nat i)) (Z.of_nat i mod 16)
+          (Vint
+             (Int.add (nthB bb i 0)
+                (Int.add
+                   (Int.add (sigma_0 (nthB bb i 1)) (sigma_1 (nthB bb i 14)))
+                   (nthB bb i 9))))) 0 LBLOCKz)
+     (eval_var _X (tarray tuint LBLOCKz)))) rearrange_regs2c
+  (normal_ret_assert
+     (EX  i0 : nat,
+      PROP  ((LBLOCK <= i0 <= c64)%nat)
+      LOCAL  (`(eq ctx) (eval_id _ctx);
+      `(eq (Vint (Int.repr (Z.of_nat i0 - 1)))) (eval_id _i);
+      `(eq
+          (map Vint
+             (rnd_64 regs K (firstn i0 (rev (generate_word (rev bb) c48))))))
+        (`cons (eval_id _a)
+           (`cons (eval_id _b)
+              (`cons (eval_id _c)
+                 (`cons (eval_id _d)
+                    (`cons (eval_id _e)
+                       (`cons (eval_id _f)
+                          (`cons (eval_id _g) (`cons (eval_id _h) `[])))))))))
+      
+      SEP  (K_vector;
+      `(array_at tuint Tsh (Xarray bb (Z.of_nat i0)) 0 LBLOCKz)
+        (eval_var _X (tarray tuint LBLOCKz))))).
+Proof.
+intros.
+simplify_Delta; abbreviate_semax.
+name a_ _a.
+name b_ _b.
+name c_ _c.
+name d_ _d.
+name e_ _e.
+name f_ _f.
+name g_ _g.
+name h_ _h.
+name T1_ _T1.
+name T2_ _T2.
+name Ki _Ki.
+name ctx_ _ctx.
+name i_ _i.
+unfold rearrange_regs2c.
+repeat forward.
+apply exp_right with (i+1)%nat.
+entailer.
+clear Delta H3.
+symmetry in H5; inv H5.
+rewrite H4; clear H4 e_.
+apply andp_right; [apply prop_right | ].
+clear TC H6 H7 ctx_ rho.
+split.
+f_equal. rewrite Nat2Z.inj_add. change (Z.of_nat 1) with 1%Z; clear; omega.
+replace (i+1)%nat with (S i) by (clear; omega); 
+ rewrite (rnd_64_S _ _ _ (nth i K Int.zero) (nth i (rev (generate_word (rev bb) 48)) Int.zero)).
+rewrite H2.
+unfold rnd_function.
+unfold map.
+f_equal.
+f_equal.
+f_equal.
+rewrite Int.add_commut.
+f_equal.
+apply nth_rev_generate_word; assumption.
+
+f_equal. f_equal. f_equal. f_equal.
+simpl. f_equal. f_equal. rewrite Int.add_commut. f_equal.
+apply nth_rev_generate_word; assumption.
+apply nth_error_nth. apply H0.
+apply nth_error_nth.
+rewrite rev_length. 
+rewrite length_generate_word; auto.
+rewrite rev_length.
+rewrite H. apply H0.
+apply sepcon_derives; auto.
+apply derives_refl'.
+apply equal_f.
+clear H6 TC ctx_ rho.
+change (Z.of_nat LBLOCK) with 16.
+apply array_at_ext; intros j ?.
+unfold upd.
+if_tac.
+subst j.
+unfold f_upto, tuints, ZnthV.
+rewrite if_false.
+rewrite (@nth_map' int val _ _ Int.zero).
+f_equal.
+
+rewrite <- (nth_rev_generate_word _ (i + 1 - LBLOCK)); auto.
+admit.  (* might even be true *)
+omega.
+rewrite rev_length, firstn_length, length_generate_word, rev_length, H.
+rewrite min_l by omega.
+apply Nat2Z.inj_lt.
+rewrite Z2Nat.id by omega. apply H3.
+clear - H3; omega.
+unfold tuints, ZnthV.
+rewrite if_false by omega.
+rewrite if_false by omega.
+rewrite (@nth_map' int val _ _ Int.zero).
+rewrite (@nth_map' int val _ _ Int.zero).
+f_equal.
+admit.  (* looks good *)
+rewrite rev_length, firstn_length, length_generate_word, rev_length, H.
+rewrite min_l by omega.
+apply Nat2Z.inj_lt.
+rewrite Z2Nat.id by omega. apply H3.
+rewrite rev_length, firstn_length, length_generate_word, rev_length, H.
+rewrite min_l by omega.
+apply Nat2Z.inj_lt.
+rewrite Z2Nat.id by omega. apply H3.
+Qed.
