sha/verif_sha_bdo6.v
@@ -1,0 +1,573 @@
+Require Import floyd.proofauto.
+Require Import sha.sha.
+Require Import sha.SHA256.
+Require Import sha.spec_sha.
+Require Import sha.sha_lemmas.
+Require Import sha.bdo_lemmas.
+Require Import sha.verif_sha_bdo5.
+Local Open Scope logic.
+
+Lemma rearrange_regs2_proof:
+ forall (Espec : OracleKind)
+   (b : list int) (ctx : val) ( regs : list int) (i : nat),
+   (length b = LBLOCK)%nat ->
+   (LBLOCK <= i < c64)%nat ->
+   (16 <= Z.of_nat i < 64) ->
+semax
+  (initialized _Ki
+     (initialized _T1
+        (initialized _t (initialized _s1 (initialized _s0 Delta_loop1)))))
+  (PROP  ()
+   LOCAL  (`(eq (Vint (nth i K Int.zero))) (eval_id _Ki);
+   `(eq
+       (Vint
+          (Int.add (nthB b i 0)
+             (Int.add
+                (Int.add (sigma_0 (nthB b i 1)) (sigma_1 (nthB b i 14)))
+                (nthB b i 9))))) (eval_id _T1); `(eq ctx) (eval_id _ctx);
+   `(eq (Vint (Int.repr (Z.of_nat i)))) (eval_id _i);
+   `(eq
+       (map Vint (rnd_64 regs K (firstn i (rev (generate_word (rev b) c48))))))
+     (`cons (eval_id _a)
+        (`cons (eval_id _b)
+           (`cons (eval_id _c)
+              (`cons (eval_id _d)
+                 (`cons (eval_id _e)
+                    (`cons (eval_id _f)
+                       (`cons (eval_id _g) (`cons (eval_id _h) `[])))))))))
+   SEP 
+   (`(array_at tuint Tsh (tuints K) 0 (Zlength K))
+      (eval_var _K256 (tarray tuint 64));
+   `(array_at tuint Tsh
+       (upd (Xarray b (Z.of_nat i)) (Z.of_nat i mod 16)
+          (Vint
+             (Int.add (nthB b i 0)
+                (Int.add
+                   (Int.add (sigma_0 (nthB b i 1)) (sigma_1 (nthB b i 14)))
+                   (nthB b i 9))))) 0 LBLOCKz)
+     (eval_var _X (tarray tuint LBLOCKz)))) rearrange_regs2b
+  (normal_ret_assert
+     (EX  i0 : nat,
+      PROP  ((LBLOCK <= i0 <= c64)%nat)
+      LOCAL  (`(eq ctx) (eval_id _ctx);
+      `(eq (Vint (Int.repr (Z.of_nat i0 - 1)))) (eval_id _i);
+      `(eq
+          (map Vint
+             (rnd_64 regs K (firstn i0 (rev (generate_word (rev b) c48))))))
+        (`cons (eval_id _a)
+           (`cons (eval_id _b)
+              (`cons (eval_id _c)
+                 (`cons (eval_id _d)
+                    (`cons (eval_id _e)
+                       (`cons (eval_id _f)
+                          (`cons (eval_id _g) (`cons (eval_id _h) `[])))))))))
+      
+      SEP  (K_vector;
+      `(array_at tuint Tsh (Xarray b (Z.of_nat i0)) 0 LBLOCKz)
+        (eval_var _X (tarray tuint LBLOCKz))))).
+Proof.
+intros.
+simplify_Delta; abbreviate_semax.
+name a_ _a.
+name b_ _b.
+name c_ _c.
+name d_ _d.
+name e_ _e.
+name f_ _f.
+name g_ _g.
+name h_ _h.
+name T1_ _T1.
+name T2_ _T2.
+name Ki _Ki.
+name ctx_ _ctx.
+name i_ _i.
+assert (LBE := LBLOCK_zeq).
+rename b into bb.
+remember (rnd_64 regs K (firstn i (rev (generate_word (rev bb) c48)))) as regs' eqn:?.
+apply (assert_LOCAL (`(exists a b c d e f g h, regs' = [a,b,c,d,e,f,g,h]))).
+clear Heqregs'.
+entailer.
+clear - H3. rename H3 into H0.
+exists a_,b_,c_,d_,e_,f_,g_,h_.
+do 8 (destruct regs' as [ | ? regs']; [inv H0 | ]).
+destruct regs'; inv H0. reflexivity.
+normalize.
+destruct H2 as [a [b [c [d [e [f [g [h H2]]]]]]]].
+rewrite Heqregs' in *. clear Heqregs'.
+rewrite H2.
+fold (@nth int).
+unfold rearrange_regs2b.
+forward. (* T1 += h + Sigma1(e) + Ch(e,f,g) + Ki; *)
+apply (assert_LOCAL (`(eq (Vint
+       (Int.add
+          (Int.add (nthB bb i 0) 
+             (Int.add (Int.add (sigma_0 (nthB bb i 1)) (sigma_1 (nthB bb i 14))) (nthB bb i 9)))
+        (Int.add (Int.add (Int.add h (Sigma_1 e)) (Ch e f g)) (nth i K Int.zero)))))
+          (eval_id _T1))).
+entailer.
+symmetry in H5; inv H5.
+f_equal. f_equal. f_equal. f_equal.
+apply Sigma_1_eq.
+apply (drop_LOCAL 1%nat); unfold delete_nth.
+apply (drop_LOCAL 2%nat); unfold delete_nth.
+clear T1_0.
+forward. 	(* T2 = Sigma0(a) + Maj(a,b,c); *)
+apply (assert_LOCAL (`(eq (Vint (Int.add (Sigma_0 a) (Maj a b c))))
+          (eval_id _T2))).
+entailer.
+symmetry in H4; inv H4.
+f_equal.
+apply Sigma_0_eq.
+apply Maj_eq.
+apply (drop_LOCAL 1%nat); unfold delete_nth.
+unfold POSTCONDITION, abbreviate; clear POSTCONDITION.
+replace Delta with (initialized _T2 (initialized _Ki (initialized _T1 (initialized _t
+                                (initialized _s1 (initialized _s0 Delta_loop1))))))
+  by (simplify_Delta; reflexivity).
+clear Delta.
+apply rearrange_regs2c_proof; assumption.
+Qed.
+
+Local Open Scope Z.
+
+Lemma sha_bdo_loop2b:
+ forall (Espec : OracleKind) (b : list int)
+    (ctx : val) (regs : list int) (i : nat) (s0 s1 : val), 
+length b = LBLOCK ->
+(LBLOCK <= i < c64)%nat ->
+16 <= Z.of_nat i < 64 ->
+semax (initialized _s1 (initialized _s0 Delta_loop1))
+  (PROP  ()
+   LOCAL  (`(eq (Vint (sigma_1 (nthB b i 14)))) (eval_id _s1);
+   `(eq (Vint (sigma_0 (nthB b i 1)))) (eval_id _s0);
+   `(eq ctx) (eval_id _ctx);
+   `(eq (Vint (Int.repr (Z.of_nat i)))) (eval_id _i);
+   `(eq
+       (map Vint (rnd_64 regs K (firstn i (rev (generate_word (rev b) c48))))))
+     (`cons (eval_id _a)
+        (`cons (eval_id _b)
+           (`cons (eval_id _c)
+              (`cons (eval_id _d)
+                 (`cons (eval_id _e)
+                    (`cons (eval_id _f)
+                       (`cons (eval_id _g) (`cons (eval_id _h) `[])))))))))
+   SEP  (K_vector;
+   `(array_at tuint Tsh (Xarray b (Z.of_nat i)) 0 LBLOCKz)
+     (eval_var _X (tarray tuint LBLOCKz))))
+  (Ssequence
+     (Sset _T1
+        (Ederef
+           (Ebinop Oadd (Evar _X (tarray tuint 16))
+              (Ebinop Oand (Etempvar _i tint) (Econst_int (Int.repr 15) tint)
+                 tint) (tptr tuint)) tuint))
+     (Ssequence
+        (Sset _t
+           (Ederef
+              (Ebinop Oadd (Evar _X (tarray tuint 16))
+                 (Ebinop Oand
+                    (Ebinop Oadd (Etempvar _i tint)
+                       (Econst_int (Int.repr 9) tint) tint)
+                    (Econst_int (Int.repr 15) tint) tint) (tptr tuint)) tuint))
+        (Ssequence
+           (Sset _T1
+              (Ebinop Oadd (Etempvar _T1 tuint)
+                 (Ebinop Oadd
+                    (Ebinop Oadd (Etempvar _s0 tuint) (Etempvar _s1 tuint)
+                       tuint) (Etempvar _t tuint) tuint) tuint))
+           (Ssequence
+              (Sassign
+                 (Ederef
+                    (Ebinop Oadd (Evar _X (tarray tuint 16))
+                       (Ebinop Oand (Etempvar _i tint)
+                          (Econst_int (Int.repr 15) tint) tint) (tptr tuint))
+                    tuint) (Etempvar _T1 tuint))
+              (Ssequence
+                 (Sset _Ki
+                    (Ederef
+                       (Ebinop Oadd (Evar _K256 (tarray tuint 64))
+                          (Etempvar _i tint) (tptr tuint)) tuint))
+                 rearrange_regs2b)))))
+  (normal_ret_assert
+     (EX  i0 : nat,
+      PROP  ((LBLOCK <= i0 <= c64)%nat)
+      LOCAL  (`(eq ctx) (eval_id _ctx);
+      `(eq (Vint (Int.repr (Z.of_nat i0 - 1)))) (eval_id _i);
+      `(eq
+          (map Vint
+             (rnd_64 regs K (firstn i0 (rev (generate_word (rev b) c48))))))
+        (`cons (eval_id _a)
+           (`cons (eval_id _b)
+              (`cons (eval_id _c)
+                 (`cons (eval_id _d)
+                    (`cons (eval_id _e)
+                       (`cons (eval_id _f)
+                          (`cons (eval_id _g) (`cons (eval_id _h) `[])))))))))
+      
+      SEP  (K_vector;
+      `(array_at tuint Tsh (Xarray b (Z.of_nat i0)) 0 LBLOCKz)
+        (eval_var _X (tarray tuint LBLOCKz))))).
+Proof.
+intros.
+simplify_Delta; abbreviate_semax.
+name a_ _a.
+name b_ _b.
+name c_ _c.
+name d_ _d.
+name e_ _e.
+name f_ _f.
+name g_ _g.
+name h_ _h.
+name T1_ _T1.
+name T2_ _T2.
+name t_ _t.
+name Ki _Ki.
+name ctx_ _ctx.
+name i_ _i.
+assert (LBE := LBLOCK_zeq).
+
+forward. (* T1 = X[i&0xf]; *) 
+clear - H H1 LBE;
+abstract (
+  entailer; 
+  replace (Int.repr (Z.of_nat i)) with (Int.repr (Z.of_nat i + 0)) by (rewrite Z.add_0_r; auto);
+  apply prop_right; split;
+   [apply X_subscript_aux; assumption | apply and_mod_15_lem]
+).
+
+apply (assert_LOCAL (`(eq (Vint (nthB b i 0))) (eval_id _T1))).
+abstract (
+ entailer; apply prop_right;
+ replace (Int.repr (Z.of_nat i)) with (Int.repr (Z.of_nat i + 0)) in H4  by (rewrite Z.add_0_r; auto);
+ rewrite X_subscript_aux2 in H3 by repable_signed;
+ replace (Z.of_nat i mod 16) with ((Z.of_nat i + 0) mod 16) in H3
+    by (rewrite Z.add_0_r; auto);
+ rewrite extract_from_b in H3 by omega;
+  clear - H3; congruence
+).
+apply (drop_LOCAL 1%nat); unfold delete_nth.
+
+forward. (* t = X[(i+9)&0xf]; *)
+clear - H H1 LBE;
+abstract (
+  entailer; apply prop_right; split;
+ [apply X_subscript_aux; assumption | apply and_mod_15_lem]).
+
+apply (assert_LOCAL (`(eq (Vint (nthB b i 9))) (eval_id _t))).
+abstract (
+ entailer; apply prop_right;
+ rewrite add_repr in H3;
+ rewrite X_subscript_aux2 in H3 by repable_signed;
+ rewrite extract_from_b in H3 by omega;
+ clear - H3; congruence).
+apply (drop_LOCAL 1%nat); unfold delete_nth.
+forward.  (* T1 += s0 + s1 + t; *)
+apply (assert_LOCAL (`(eq (Vint (Int.add (nthB b i 0)
+                         (Int.add (Int.add (sigma_0 (nthB b i 1))
+                                                   (sigma_1 (nthB b i 14)))
+                                      (nthB b i 9))))) (eval_id _T1))).
+ abstract entailer.
+apply (drop_LOCAL 1%nat); unfold delete_nth.
+apply (drop_LOCAL 1%nat); unfold delete_nth.
+apply (drop_LOCAL 1%nat); unfold delete_nth.
+apply (drop_LOCAL 1%nat); unfold delete_nth.
+apply (drop_LOCAL 1%nat); unfold delete_nth.
+ clear s0 s1 T1_0.
+
+forward. (* X[i&0xf] = T1; *)
+instantiate (2:= (Z.of_nat i  mod 16)).
+instantiate (1:=  (Vint (Int.add (nthB b i 0)
+                         (Int.add (Int.add (sigma_0 (nthB b i 1))
+                                                   (sigma_1 (nthB b i 14)))
+                                      (nthB b i 9))))).
+abstract (
+ entailer;
+ apply prop_right; split;
+ [ unfold Int.and; rewrite mul_repr;
+  f_equal; f_equal; f_equal; 
+  change (Int.unsigned (Int.repr 15)) with (Z.ones 4);
+  rewrite Z.land_ones by (clear; omega);
+  f_equal; rewrite Int.unsigned_repr by repable_signed; auto
+ | change LBLOCKz with 16; apply Z.mod_bound_pos; omega
+ ]).
+
+unfold K_vector.
+forward.  (* Ki=K256[i]; *)
+abstract (
+ entailer; split;
+ [unfold tuints, ZnthV; rewrite if_false by (clear; omega);
+ rewrite (@nth_map' int val _ _ Int.zero); [apply I | ];
+ change (length K) with 64%nat; rewrite Nat2Z.id; destruct H0 as [_ H0]; apply H0
+ | change (Zlength K) with 64; destruct H1; assumption]).
+
+apply (assert_LOCAL (`(eq (Vint (nth i K Int.zero))) (eval_id _Ki))).
+entailer.
+rewrite Int.signed_repr in H3 by repable_signed.
+unfold tuints, ZnthV in H3.
+rewrite if_false in H3 by omega.
+rewrite Nat2Z.id in H3.
+rewrite (@nth_map' int val _ _ Int.zero) in H3.
+injection H3; clear; auto.
+clear - H0. apply H0.
+apply (drop_LOCAL 1%nat); unfold delete_nth.
+
+unfold POSTCONDITION, abbreviate; clear POSTCONDITION.
+replace Delta with (initialized _Ki (initialized _T1 (initialized _t
+                                (initialized _s1 (initialized _s0 Delta_loop1)))))
+  by (simplify_Delta; reflexivity).
+clear Delta.
+apply rearrange_regs2_proof; assumption.
+Admitted. (* Proof is done here, Qed takes more than 2 gigs *)
+*)
+
+Lemma bdo_loop2_body_proof:
+ forall (Espec : OracleKind)
+   (b : list int) (ctx : val) ( regs : list int) (i : nat)
+   (H : length b = LBLOCK)
+   (H0 : (LBLOCK <= i < c64)%nat),
+semax Delta_loop1
+  (PROP  ()
+   LOCAL  (`(eq ctx) (eval_id _ctx);
+   `(eq (Vint (Int.repr (Z.of_nat i)))) (eval_id _i);
+   `(eq
+       (map Vint (rnd_64 regs K (firstn i (rev (generate_word (rev b) c48))))))
+     (`cons (eval_id _a)
+        (`cons (eval_id _b)
+           (`cons (eval_id _c)
+              (`cons (eval_id _d)
+                 (`cons (eval_id _e)
+                    (`cons (eval_id _f)
+                       (`cons (eval_id _g) (`cons (eval_id _h) `[])))))))))
+   SEP  (K_vector;
+   `(array_at tuint Tsh (Xarray b (Z.of_nat i)) 0 LBLOCKz)
+     (eval_var _X (tarray tuint LBLOCKz)))) bdo_loop2_body
+  (normal_ret_assert
+     (EX  i0 : nat,
+      PROP  (LBLOCK <= i0 <= c64)
+      LOCAL  (`(eq ctx) (eval_id _ctx);
+      `(eq (Vint (Int.repr (Z.of_nat i0 - 1)))) (eval_id _i);
+      `(eq
+          (map Vint
+             (rnd_64 regs K (firstn i0 (rev (generate_word (rev b) c48))))))
+        (`cons (eval_id _a)
+           (`cons (eval_id _b)
+              (`cons (eval_id _c)
+                 (`cons (eval_id _d)
+                    (`cons (eval_id _e)
+                       (`cons (eval_id _f)
+                          (`cons (eval_id _g) (`cons (eval_id _h) `[])))))))))
+      
+      SEP  (K_vector;
+      `(array_at tuint Tsh (Xarray b (Z.of_nat i0)) 0 LBLOCKz)
+        (eval_var _X (tarray tuint LBLOCKz))))).
+Proof.
+intros.
+simplify_Delta; unfold bdo_loop2_body; abbreviate_semax.
+name a_ _a.
+name b_ _b.
+name c_ _c.
+name d_ _d.
+name e_ _e.
+name f_ _f.
+name g_ _g.
+name h_ _h.
+name t_ _t.
+name Ki _Ki.
+name ctx_ _ctx.
+name i_ _i.
+assert (LBE := LBLOCK_zeq).
+assert (16 <= Z.of_nat i < 64)%Z. {
+ destruct H0.
+ apply Nat2Z.inj_le in H0.
+ apply Nat2Z.inj_lt in H1.
+ change (Z.of_nat c64) with 64%Z in H1.
+ omega.
+}
+
+forward.	(*s0 = X[(i+1)&0x0f]; *)
+entailer; apply prop_right; split;
+ [ apply X_subscript_aux; assumption | apply and_mod_15_lem].
+
+forward. (* s0 = sigma0(s0); *)
+rename x into s0'.
+
+
+
+apply (assert_LOCAL (`(eq (Vint (sigma_0 (nthB b i 1)))) (eval_id _s0))).
+entailer; apply prop_right. 
+rewrite add_repr in H3.
+rewrite X_subscript_aux2 in H3 by repable_signed.
+
+
+
+rewrite extract_from_b in H3 by omega.
+simpl in H3.
+rewrite Int.and_mone in H3.
+inv H3.
+apply sigma_0_eq.
+apply (drop_LOCAL 1%nat); unfold delete_nth.
+apply (drop_LOCAL 1%nat); unfold delete_nth.
+clear s0'.
+
+forward. (* s1 = X[(i+14)&0x0f]; *)
+entailer; apply prop_right; split;
+ [apply X_subscript_aux; assumption | apply and_mod_15_lem].
+forward. (* s1 = sigma1(s1); *)
+rename x into s1'.
+
+apply (assert_LOCAL (`(eq (Vint (sigma_1 (nthB b i 14)))) (eval_id _s1))).
+entailer; apply prop_right. 
+rewrite add_repr in H3.
+rewrite X_subscript_aux2 in H3 by repable_signed.
+rewrite extract_from_b in H3 by omega.
+simpl in H3.
+rewrite Int.and_mone in H3.
+inv H3.
+apply sigma_1_eq.
+apply (drop_LOCAL 1%nat); unfold delete_nth.
+apply (drop_LOCAL 1%nat); unfold delete_nth.
+clear s1'.
+
+unfold MORE_COMMANDS, POSTCONDITION, abbreviate; clear MORE_COMMANDS POSTCONDITION.
+replace Delta with (initialized _s1 (initialized _s0 Delta_loop1))
+  by (simplify_Delta; reflexivity).
+clear Delta.
+apply sha_bdo_loop2b; assumption.
+Qed.
+*)
+
+Lemma sha256_block_data_order_loop2_proof:
+  forall (Espec : OracleKind)
+     (b: list int) ctx (regs: list int),
+     length b = LBLOCK ->
+     semax  Delta_loop1
+ (PROP ()
+   LOCAL (`(eq ctx) (eval_id _ctx);
+               `(eq (Vint (Int.repr 16))) (eval_id _i);
+                `(eq (map Vint (rnd_64 regs K b))) 
+                   (`cons (eval_id _a) (`cons (eval_id _b) (`cons (eval_id _c) (`cons (eval_id _d)
+                     (`cons (eval_id _e) (`cons (eval_id _f) (`cons (eval_id _g) (`cons (eval_id _h) `nil)))))
+))))
+   SEP ( K_vector;
+           `(array_at tuint Tsh (tuints b) 0 16) (eval_var _X (tarray tuint 16))))
+  block_data_order_loop2
+  (normal_ret_assert
+    (PROP () 
+     LOCAL(`(eq ctx) (eval_id _ctx);
+                `(eq (map Vint (rnd_64 regs K (rev (generate_word (rev b) 48)))))
+                   (`cons (eval_id _a) (`cons (eval_id _b) (`cons (eval_id _c) (`cons (eval_id _d)
+                     (`cons (eval_id _e) (`cons (eval_id _f) (`cons (eval_id _g) (`cons (eval_id _h) `nil)))))
+))))
+     SEP (K_vector;
+           `(array_at_ tuint Tsh 0 16) (eval_var _X (tarray tuint 16))))).
+Proof.
+intros.
+unfold block_data_order_loop2; simpl nth.
+fold rearrange_regs2c.
+fold rearrange_regs2b.
+fold bdo_loop2_body.
+abbreviate_semax.
+name a_ _a.
+name b_ _b.
+name c_ _c.
+name d_ _d.
+name e_ _e.
+name f_ _f.
+name g_ _g.
+name h_ _h.
+name t_ _t.
+name Ki _Ki.
+name ctx_ _ctx.
+name i_ _i.
+change 16%nat with LBLOCK.
+
+Definition loop2_inv (rg0: list int) (b: list int) ctx  (delta: Z) (i: nat) :=
+    PROP ( (LBLOCK <= i <= c64)%nat )
+    LOCAL  (`(eq ctx) (eval_id _ctx); 
+                 `(eq (Vint (Int.repr (Z.of_nat i - delta)))) (eval_id _i);
+     `(eq (map Vint (rnd_64 rg0 K (firstn i ((rev(generate_word (rev b) c48)))))))
+      (`cons (eval_id _a)
+         (`cons (eval_id _b)
+            (`cons (eval_id _c)
+               (`cons (eval_id _d)
+                  (`cons (eval_id _e)
+                     (`cons (eval_id _f)
+                        (`cons (eval_id _g) (`cons (eval_id _h) `[])))))))))
+     SEP (K_vector;
+    `(array_at tuint Tsh (Xarray b (Z.of_nat i)) 0 LBLOCKz)
+           (eval_var _X (tarray tuint LBLOCKz))).
+
+apply semax_pre with (EX i:nat, loop2_inv regs b ctx 0 i).
+clear POSTCONDITION; 
+abstract(
+ unfold loop2_inv;  apply exp_right with LBLOCK;
+ change LBLOCKz with 16%Z;
+  change (Z.of_nat LBLOCK) with LBLOCKz;
+ rewrite array_at_Xarray by auto;
+  entailer!;
+  [change LBLOCK with 16%nat; change c64 with 64%nat; clear; omega
+  | rewrite generate_word_lemma1; auto]
+).
+
+apply semax_post' with (loop2_inv regs b ctx 0 c64). 
+change 48%nat with c48.
+clear POSTCONDITION; 
+abstract (
+ unfold loop2_inv;
+ entailer;
+ rewrite firstn_same in H2
+  by(rewrite rev_length, length_generate_word, rev_length, H;
+      change (64>=64)%nat; auto);
+ rewrite prop_true_andp by auto;
+  cancel).
+
+apply (semax_loop _ _ (EX i:nat, loop2_inv regs b ctx 1 i)).
+2: abstract (
+apply extract_exists_pre; intro i;
+forward;  (*  i += 1; *)
+apply exp_right with i;
+ unfold loop2_inv;  entailer! ; f_equal; omega).
+
+apply extract_exists_pre; intro i.
+unfold loop2_inv.
+repeat rewrite Z.sub_0_r.
+
+forward_if (
+   PROP  ((LBLOCK <= i < c64)%nat)
+   LOCAL  (`(eq ctx) (eval_id _ctx);
+   `(eq (Vint (Int.repr (Z.of_nat i)))) (eval_id _i);
+   `(eq
+       (map Vint (rnd_64 regs K (firstn i (rev (generate_word (rev b) c48))))))
+     (`cons (eval_id _a)
+        (`cons (eval_id _b)
+           (`cons (eval_id _c)
+              (`cons (eval_id _d)
+                 (`cons (eval_id _e)
+                    (`cons (eval_id _f)
+                       (`cons (eval_id _g) (`cons (eval_id _h) `[])))))))))
+   SEP  (K_vector;
+   `(array_at tuint Tsh (Xarray b (Z.of_nat i)) 0 LBLOCKz)
+     (eval_var _X (tarray tuint LBLOCKz)))).
+ abstract entailer.
+ forward; (* skip *)
+   assert (LBE : LBLOCKz=16%Z) by reflexivity; change c64 with 64%nat in *; entailer. 
+ (* change (Z.of_nat c64) with 64. *)
+   apply semax_extract_PROP; intro;
+   assert (LBE : LBLOCKz=16%Z) by reflexivity; change c64 with 64%nat in *;
+   forward; (* break; *)
+   cbv beta.
+  change 64%nat with c64.
+(*  change (Z.of_nat c64) with 64%Z. *)
+  entailer.
+   assert (i=64)%nat by omega; subst i;
+   apply andp_right; [ apply prop_right | cancel].
+ split; auto. change (16<=64)%nat; clear; omega.
+unfold POSTCONDITION, abbreviate; clear POSTCONDITION.
+
+make_sequential. rewrite loop1_ret_assert_normal.
+normalize.
+replace Delta with
+  (Delta_loop1) by (simplify_Delta; reflexivity).
+
+apply bdo_loop2_body_proof; auto.
+Qed.
+
