Makefile
@@ -150,7 +150,8 @@ SHA_FILES= \
   SHA256.v sha_lemmas.v sha_lemmas2.v \
   sha.v spec_sha.v verif_sha_init.v \
   verif_sha_update.v verif_sha_update2.v verif_sha_update3.v verif_sha_update4.v \
-  verif_sha_bdo.v verif_sha_bdo2.v verif_sha_bdo3.v verif_sha_bdo4.v \
+  bdo_lemmas.v verif_sha_bdo.v verif_sha_bdo2.v verif_sha_bdo3.v \
+  verif_sha_bdo4.v verif_sha_bdo5.v verif_sha_bdo6.v \
   verif_sha_final2.v verif_sha_final3.v verif_sha_final.v \
   verif_addlength.v verif_SHA256.v entail_examples2.v 
 
@@ -243,7 +244,7 @@ count:
 count-linking:
 	wc $(LINKING_FILES:%.v=linking/%.v)
 
-$(CC_TARGET): compcert/make
-	(cd compcert; ./make)
+# $(CC_TARGET): compcert/make
+#	(cd compcert; ./make)
 
 include .depend
